src/Set.fst
@@ -8,6 +8,7 @@ type set (a:Type) = a -> Tot bool
 
 val mem          : #a:Type -> a -> set a -> Tot bool
 val empty        : #a:Type -> Tot (set a)
+val full         : #a:Type -> Tot (set a)
 val singleton    : #a:Type -> a -> Tot (set a)
 val union        : #a:Type -> set a -> set a -> Tot (set a)
 val intersection : #a:Type -> set a -> set a -> Tot (set a)
@@ -16,6 +17,7 @@ val ins          : #a:Type -> a -> set a -> Tot (set a)
 
 let mem i s          = s i
 let empty            = fun _ -> false
+let full             = fun _ -> true
 let singleton a      = fun b -> b = a
 let union a b        = fun c -> a c || b c
 let intersection a b = fun c -> a c && b c
