src/Total.fst
@@ -66,24 +66,32 @@ val agree_on_trans : #key:Type -> #value:Type -> m:t key value -> m':t key value
 let agree_on_trans m m' m'' s = ()
 
 
-(* Functional extensionality for lookups *)
-open FStar.FunctionalExtensionality
+(* Functional extensionality for lookups. We're rolling our own since we're
+going to be bad and assume maps which are extensionally equal are actually equal *)
 
-type Equal (#key:Type) (#value:Type) (m1:t key value) (m2:t key value) = FEq (lookup m1) (lookup m2)
+type Equal (#key:Type) (#value:Type) (m1:t key value) (m2:t key value) = 
+  (forall x.{:pattern (lookup m1 x) \/ (lookup m2 x)} lookup m1 x = lookup m2 x)
+
+(* What did they say about assumption being the mother of all fuckups? *)
+assume TotalExtensionality : 
+  forall (key:Type) (value:Type) (m1:t key value) (m2:t key value).
+    {:pattern Equal m1 m2} Equal m1 m2 <==> m1 = m2
+
 val lemma_map_equal_intro: #key:Type -> #value:Type -> m1:t key value -> m2:t key value ->
   Lemma (requires  (forall x. lookup m1 x = lookup m2 x))
         (ensures   (Equal m1 m2))
   [SMTPatT (Equal m1 m2)]
 val lemma_map_equal_elim: #key:Type -> #value:Type -> m1:t key value -> m2:t key value ->
   Lemma (requires (Equal m1 m2))
-        (ensures  (lookup m1 = lookup m2))
+        (ensures  (m1 = m2))
   [SMTPatT (Equal m1 m2)]
 val lemma_map_equal_refl: #key:Type -> #value:Type -> m1:t key value -> m2:t key value ->
-  Lemma (requires (lookup m1 = lookup m2))
+  Lemma (requires (m1 = m2))
         (ensures  (Equal m1 m2))
   [SMTPatT (Equal m1 m2)]
 
 let lemma_map_equal_intro m1 m2 = ()
-let lemma_map_equal_elim m1 m2 = ()
+(* Follows from TotalExtensionality but I can't seem to get it working *)
+let lemma_map_equal_elim m1 m2 = admit()
 let lemma_map_equal_refl m1 m2 = ()
 
