src/TypeCheck.fst
@@ -1,0 +1,395 @@
+(** Type checker *)
+module TypeCheck
+
+(* Type checking is really a misnomer -- we don't type check
+   in the sense of preventing run-time errors. Type checking
+   in ReVer is really a static analysis to infer array bounds
+   and allow the compiler to allocate space for every
+   register statically. Type inference serves as a useful
+   way to frame the problem, with the added benefit that the
+   framework may be used later to better effect when features
+   are added *)
+
+open Partial
+open ExprTypes
+
+type ctxt = Par.map string GType
+
+type wellTypedCtxt : ctxt -> string -> GType -> Type =
+  | Ctxt_zero : s:string -> ty:GType -> xs:ctxt -> wellTypedCtxt ((s, ty)::xs) s ty
+  | Ctxt_succ : s:string -> ty:GType -> x:(string * GType){~(fst x = s)} -> xs:ctxt ->
+                wellTypedCtxt xs s ty ->
+                wellTypedCtxt (x::xs) s ty
+
+type subType : GType -> GType -> Type =
+  | Sub_refl : #t1:GType -> subType t1 t1
+  | Sub_arry : n:nat -> m:fin n -> subType (GArray n) (GArray m)
+  | Sub_lam  : #t1:GType -> #t2:GType -> #s1:GType -> #s2:GType ->
+               subType s1 t1 ->
+               subType t2 s2 ->
+               subType (GFun (t1, t2)) (GFun (s1, s2))
+
+type wellTyped : ctxt -> GExpr -> GType -> Type =
+  | Wt_let : #ctx:ctxt -> #s:string -> #t1:GExpr -> #t2:GExpr -> #ty1:GType -> #ty2:GType ->
+             wellTyped ctx t1 ty1 ->
+             wellTyped ((s, ty1)::ctx) t2 ty2 ->
+             wellTyped ctx (LET (s, t1, t2)) ty2
+  | Wt_lam : #ctx:ctxt -> #s:string -> #ty1:GType -> #t:GExpr -> #ty2:GType ->
+             wellTyped ((s, ty1)::ctx) t ty2 ->
+             wellTyped ctx (LAMBDA (s, ty1, t)) (GFun (ty1, ty2))
+  | Wt_apl : #ctx:ctxt -> #t1:GExpr -> #t2:GExpr -> #ty1:GType -> #ty2:GType -> #ty3:GType ->
+             wellTyped ctx t1 (GFun (ty1, ty2)) ->
+             wellTyped ctx t2 ty3 ->
+             subType ty3 ty1 ->
+             wellTyped ctx (APPLY (t1, t2)) ty2
+  | Wt_ite : #ctx:ctxt -> #t1:GExpr -> #t2:GExpr -> #t3:GExpr -> #ty1:GType -> #ty2:GType -> #ty3:GType ->
+             wellTyped ctx t1 GBool ->
+             wellTyped ctx t2 ty1 ->
+             wellTyped ctx t3 ty2 ->
+             subType ty1 ty3 ->
+             subType ty2 ty3 ->
+             wellTyped ctx (IFTHENELSE (t1, t2, t3)) ty3
+  | Wt_seq : #ctx:ctxt -> #t1:GExpr -> #t2:GExpr -> #ty:GType ->
+             wellTyped ctx t1 GUnit ->
+             wellTyped ctx t2 ty ->
+             wellTyped ctx (SEQUENCE (t1, t2)) ty
+  | Wt_ass : #ctx:ctxt -> #t1:GExpr -> #t2:GExpr ->
+             wellTyped ctx t1 GBool ->
+             wellTyped ctx t2 GBool ->
+             wellTyped ctx (ASSIGN (t1, t2)) GUnit
+  | Wt_unt : #ctx:ctxt -> wellTyped ctx UNIT GUnit
+  | Wt_xor : #ctx:ctxt -> #t1:GExpr -> #t2:GExpr ->
+             wellTyped ctx t1 GBool ->
+             wellTyped ctx t2 GBool ->
+             wellTyped ctx (XOR (t1, t2)) GBool
+  | Wt_and : #ctx:ctxt -> #t1:GExpr -> #t2:GExpr ->
+             wellTyped ctx t1 GBool ->
+             wellTyped ctx t2 GBool ->
+             wellTyped ctx (AND (t1, t2)) GBool
+  | Wt_bl  : #ctx:ctxt -> b:bool -> wellTyped ctx (BOOL b) GBool
+  | Wt_apn : #ctx:ctxt -> #t1:GExpr -> #t2:GExpr -> #n:nat -> #m:nat ->
+             wellTyped ctx t1 (GArray n) ->
+             wellTyped ctx t2 (GArray m) ->
+             wellTyped ctx (APPEND (t1, t2)) (GArray (n + m))
+  | Wt_rot : #ctx:ctxt -> #t:GExpr -> #n:nat -> i:fin n ->
+             wellTyped ctx t (GArray n) ->
+             wellTyped ctx (ROT (i, t)) (GArray n)
+  | Wt_slc : #ctx:ctxt -> #t:GExpr -> #n:nat -> i:nat -> j:nat{i <= j && j < n} ->
+             wellTyped ctx t (GArray n) ->
+             wellTyped ctx (SLICE (t, i, j)) (GArray (j - i))
+  | Wt_arz : #ctx:ctxt -> wellTyped ctx (ARRAY []) (GArray 0)
+  | Wt_ars : #ctx:ctxt -> #t:GExpr -> #ts:list GExpr -> #n:nat ->
+             wellTyped ctx t GBool ->
+             wellTyped ctx (ARRAY ts) (GArray n) ->
+             wellTyped ctx (ARRAY (t::ts)) (GArray (n+1))
+  | Wt_gta : #ctx:ctxt -> #t:GExpr -> #n:nat -> i:fin n ->
+             wellTyped ctx t (GArray n) ->
+             wellTyped ctx (GET_ARRAY (t, i)) GBool
+  | Wt_get : #ctx:ctxt -> #s:string -> #ty:GType ->
+             wellTypedCtxt ctx s ty ->
+             wellTyped ctx (VAR s) ty
+  | Wt_ast : #ctx:ctxt -> #t:GExpr ->
+             wellTyped ctx t GBool ->
+             wellTyped ctx (ASSERT t) GUnit
+  | Wt_loc : #ctx:ctxt -> i:int ->
+             wellTyped ctx (LOC i) GBool
+  | Wt_bex : #ctx:ctxt -> bexp:BoolExp ->
+             wellTyped ctx (BEXP bexp) GBool
+
+val subtype : t1:GType -> t2:GType -> Tot bool
+val suptype : t1:GType -> t2:GType -> Tot bool
+let rec subtype t1 t2 = if t1 = t2 then true else match (t1, t2) with
+  | (GArray i, GArray j) -> j <= i
+  | (GFun (t1, t2), GFun (s1, s2)) -> (suptype t1 s1) && (subtype t2 s2)
+  | _ -> false
+and suptype t1 t2 = if t1 = t2 then true else match (t1, t2) with
+  | (GArray i, GArray j) -> j >= i
+  | (GFun (t1, t2), GFun (s1, s2)) -> (subtype t1 s1) && (suptype t2 s2)
+  | _ -> false
+
+val welltyctx_imp_findctx : ctx:ctxt -> s:string -> ty:GType -> wellTypedCtxt ctx s ty ->
+  Lemma (find ctx s = Some ty)
+let rec welltyctx_imp_findctx ctx s ty h = match h with
+  | Ctxt_zero s ty xs -> ()
+  | Ctxt_succ s ty x xs h' -> welltyctx_imp_findctx xs s ty h'
+
+val findctx_imp_welltyctx : ctx:ctxt -> s:string -> ty:GType -> h:unit{find ctx s = Some ty} ->
+  wellTypedCtxt ctx s ty
+let rec findctx_imp_welltyctx ctx s ty h = match ctx with
+  | (x,y)::xs -> if x = s && y = ty
+    then Ctxt_zero s ty xs
+    else Ctxt_succ s ty (x,y) xs (findctx_imp_welltyctx xs s ty ())
+
+(* Type inference *)
+type IExp =
+  | ILit   of int
+  | IVar   of int
+  | IPlus  of IExp * IExp
+  | IMinus of IExp
+
+type TyExp =
+  | TUnit
+  | TBool
+  | TVar   of int
+  | TArray of IExp
+  | TArrow of TyExp * TyExp
+
+val normalize : IExp -> IExp
+let rec normalize iexp = match iexp with
+  | IMinus x ->
+    begin match normalize x with
+      | IMinus x'    -> x'
+      | ILit i       -> ILit (-i)
+      | IPlus (x, y) -> IPlus (normalize (IMinus x), normalize (IMinus y))
+      | x'           -> IMinus x'
+    end
+  | IPlus (x, y) ->
+    begin match (normalize x, normalize y) with
+      | (IVar i, y') | (y', IVar i)       -> IPlus (IVar i, y')
+      | (ILit i, ILit j)                  -> ILit (i+j)
+      | (IPlus (IVar i, x'), y')
+      | (y', IPlus (IVar i, x'))          -> IPlus (IVar i, IPlus (x', y'))
+      | (IPlus (IMinus (IVar i), x'), y')
+      | (y', IPlus (IMinus (IVar i), x')) -> IPlus (IMinus (IVar i), IPlus (x', y'))
+      | (x', y')                          -> IPlus (x', y')
+    end
+  | _ -> iexp
+
+val toTyExp : GType -> Tot TyExp
+let rec toTyExp ty = match ty with
+  | GUnit -> TUnit
+  | GBool -> TBool
+  | GVar i -> TVar i
+  | GArray n -> TArray (ILit n)
+  | GFun (ty1, ty2) -> TArrow (toTyExp ty1, toTyExp ty2)
+
+val toGType : TyExp -> GType
+let rec toGType texp = match texp with
+  | TUnit -> GUnit
+  | TBool -> GBool
+  | TVar i -> GVar i
+  | TArray iexp ->
+    begin match normalize iexp with
+      | ILit n -> GArray n
+      | _ -> GArray 0
+    end
+  | TArrow (texp1, texp2) -> GFun (toGType texp1, toGType texp2)
+
+(* Constraints (equality or less than) over type expressions *)
+type Cons =
+  | ICons of IExp * IExp
+  | TCons of TyExp * TyExp
+
+type ctxt' = map string TyExp
+
+val inferTypes : int -> ctxt' -> tm:GExpr -> Tot (int * list Cons * list Cons * TyExp) (decreases %[tm;0])
+val inferTypes_lst : int -> ctxt' -> l:list GExpr -> Tot (int * list Cons * list Cons) (decreases %[l;1])
+let rec inferTypes top ctx gexp = match gexp with
+  | LET (x, t1, t2) ->
+    let (top', ec1, lc1, ty1) = inferTypes top ctx t1 in
+    let (top'', ec2, lc2, ty2) = inferTypes top' ((x, ty1)::ctx) t2 in
+        (top'', ec1@ec2, lc1@lc2, ty2)
+  | LAMBDA (x, ty, t) ->
+    let (top', ec1, lc1, ty1) = inferTypes top ((x, (toTyExp ty))::ctx) t in
+        (top', ec1, lc1, TArrow (toTyExp ty, ty1))
+  | APPLY (t1, t2) ->
+    let (top', ec1, lc1, ty1) = inferTypes top ctx t1 in
+    let (top'', ec2, lc2, ty2) = inferTypes top' ctx t2 in
+    let e = TCons (ty1, TArrow (TVar top'', TVar (top''+1))) in
+    let c = TCons (ty2, TVar top'') in
+      (top''+2, e::(ec1@ec2), c::(lc1@lc2), TVar (top''+1))
+  | IFTHENELSE (t1, t2, t3) ->
+    let (top', ec1, lc1, ty1) = inferTypes top ctx t1 in
+    let (top'', ec2, lc2, ty2) = inferTypes top' ctx t2 in
+    let (top''', ec3, lc3, ty3) = inferTypes top'' ctx t3 in
+    let e1 = TCons (ty1, TBool) in
+    let e2 = TCons (ty2, TVar top''') in
+    let e3 = TCons (ty3, TVar top''') in
+      (top'''+1, e1::e2::e3::(ec1@ec2@ec3), lc1@lc2, TVar top''')
+  | SEQUENCE (t1, t2) ->
+    let (top', ec1, lc1, ty1) = inferTypes top ctx t1 in
+    let (top'', ec2, lc2, ty2) = inferTypes top' ctx t2 in
+    let e1 = TCons (ty1, TUnit) in
+      (top'', e1::(ec1@ec2), lc1@lc2, ty2)
+  | ASSIGN (t1, t2) ->
+    let (top', ec1, lc1, ty1) = inferTypes top ctx t1 in
+    let (top'', ec2, lc2, ty2) = inferTypes top' ctx t2 in
+    let e1 = TCons (ty1, TBool) in
+    let e2 = TCons (ty2, TBool) in
+      (top'', e1::e2::(ec1@ec2), lc1@lc2, TUnit)
+  | VAR x -> begin match Par.find ctx x with
+    | None -> (top, [], [], TUnit)
+    | Some ty -> (top, [], [], ty)
+  end
+  | UNIT -> (top, [], [], TUnit)
+  | BOOL b -> (top, [], [], TBool)
+  | XOR (t1, t2) | AND (t1, t2) ->
+    let (top', ec1, lc1, ty1) = inferTypes top ctx t1 in
+    let (top'', ec2, lc2, ty2) = inferTypes top' ctx t2 in
+    let e1 = TCons (ty1, TBool) in
+    let e2 = TCons (ty2, TBool) in
+      (top'', e1::e2::(ec1@ec2), lc1@lc2, TBool)
+  | ARRAY tlst ->
+    let (top', ec, lc) = inferTypes_lst top ctx tlst in
+      (top', ec, lc, TArray (ILit (FStar.List.lengthT tlst)))
+  | GET_ARRAY (t, i) ->
+    let (top', ec1, lc1, ty1) = inferTypes top ctx t in
+    let e1 = TCons (ty1, TArray (IVar top')) in
+    let l1 = ICons (ILit i, IVar top') in
+      (top'+1, e1::ec1, l1::lc1, TBool)
+  | APPEND (t1, t2) ->
+    let (top', ec1, lc1, ty1) = inferTypes top ctx t1 in
+    let (top'', ec2, lc2, ty2) = inferTypes top' ctx t2 in
+    let e1 = TCons (ty1, TArray (IVar top'')) in
+    let e2 = TCons (ty2, TArray (IVar (top''+1))) in
+    let e3 = ICons (IVar (top''+2), IPlus (IVar top'', IVar (top''+1))) in
+      (top''+3, e1::e2::e3::(ec1@ec2), lc1@lc2, TArray (IVar (top''+2)))
+  | ROT (i, t) ->
+    let (top', ec1, lc1, ty1) = inferTypes top ctx t in
+    let e1 = TCons (ty1, TArray (IVar top')) in
+    let l1 = ICons (ILit (i+1), IVar top') in
+      (top'+1, e1::ec1, l1::lc1, TArray (IVar top'))
+  | SLICE (t, i, j) ->
+    let (top', ec1, lc1, ty1) = inferTypes top ctx t in
+    let e1 = TCons (ty1, TArray (IVar top')) in
+    let l1 = ICons (ILit (j+1), IVar top') in
+      (top'+1, e1::ec1, l1::lc1, TArray (ILit (j - i + 1)))
+  | ASSERT t ->
+    let (top', ec1, lc1, ty1) = inferTypes top ctx t in
+    let e1 = TCons (ty1, TBool) in
+      (top', e1::ec1, lc1, TUnit)
+  | LOC i -> (top, [], [], TBool)
+  | BEXP bexp -> (top, [], [], TBool)
+  | _ -> (top, [], [], TUnit)
+and inferTypes_lst top ctx lst = match lst with
+  | [] -> (top, [], [])
+  | x::xs ->
+    let (top', ec1, lc1, ty1) = inferTypes top ctx x in
+    let (top'', ec2, lc2) = inferTypes_lst top' ctx xs in
+    let e1 = TCons (ty1, TBool) in
+      (top'', e1::(ec1@ec2), lc1@lc2)
+
+
+let rec substIExp i iexp x = match x with
+  | ILit j -> ILit j
+  | IVar j -> if i = j then iexp else IVar j
+  | IMinus x -> substIExp i iexp x
+  | IPlus (x, y) -> IPlus (substIExp i iexp x, substIExp i iexp y)
+
+let rec substTExp i texp x = match x with
+  | TUnit -> TUnit
+  | TBool -> TBool
+  | TVar j -> if i = j then texp else TVar j
+  | TArray iexp -> TArray iexp
+  | TArrow (x, y) -> TArrow (substTExp i texp x, substTExp i texp y)
+
+let rec substIExpInTExp i iexp x = match x with
+  | TArray iexp' -> TArray (substIExp i iexp iexp')
+  | TArrow (x, y) -> TArrow (substIExpInTExp i iexp x, substIExpInTExp i iexp y)
+  | _ -> x
+
+let rec iSubst i iexp cons = match cons with
+  | [] -> []
+  | (ICons (c1, c2))::xs -> (ICons (substIExp i iexp c1, substIExp i iexp c2))::(iSubst i iexp xs)
+  | (TCons (c1, c2))::xs -> (TCons (substIExpInTExp i iexp c1, substIExpInTExp i iexp c2))::(iSubst i iexp xs)
+
+let rec tSubst i texp cons = match cons with
+  | [] -> []
+  | (TCons c)::xs -> (TCons (substTExp i texp (fst c), substTExp i texp (snd c)))::(tSubst i texp xs)
+  | x::xs -> x::(tSubst i texp xs)
+
+let rec mergeLower iexp j bnds = match bnds with
+  | [] -> Some iexp
+  | (ICons (iexp', IVar h))::xs -> 
+    if h = j then 
+      begin match (normalize iexp, normalize iexp') with
+        | (ILit x, ILit y) -> mergeLower (ILit (max x y)) j xs
+        | (IVar x, IVar y) -> if x = y then mergeLower (IVar x) j xs else None
+        | _ -> None
+      end
+    else 
+      mergeLower iexp j xs
+  | _::xs -> mergeLower iexp j xs
+
+let rec unify_bnds top bnds subs = 
+  match bnds with
+  | [] -> Some subs
+  | (ICons (i1, i2))::xs ->
+    begin match (normalize i1, normalize i2) with
+      | (iexp, IVar j) ->
+        begin match (mergeLower iexp j xs) with
+          | Some sub -> unify_bnds top (iSubst j sub xs) (iSubst j sub subs)
+          | None -> unify_bnds top (xs @ [ICons (iexp, IVar j)]) subs
+        end
+      | (ILit x, ILit y) -> if x <= y then unify_bnds top xs subs else None
+      | (iexp, iexp') -> unify_bnds top (xs @ [ICons (iexp, iexp')]) subs
+    end
+  | (TCons (t1, t2))::xs ->
+    begin match (t1, t2) with
+      | (TVar i, TUnit) | (TUnit, TVar i) -> unify_bnds top (tSubst i TUnit xs) (tSubst i TUnit subs)
+      | (TVar i, TBool) | (TBool, TVar i) -> unify_bnds top (tSubst i TBool xs) (tSubst i TBool subs)
+      | (TVar i, TArray iexp) -> 
+          let sub = TArray (IVar top) in
+            unify_bnds (top+1) 
+                       (tSubst i sub ((ICons (iexp, IVar top))::xs)) 
+                       ((TCons (TVar i, sub))::(tSubst i sub subs))
+      | (TArray iexp, TVar i) -> 
+          let sub = TArray (IVar top) in
+            unify_bnds (top+1) 
+                       (tSubst i sub ((ICons (IVar top, iexp))::xs)) 
+                       ((TCons (TVar i, sub))::(tSubst i sub subs))
+      | (TVar i, TArrow (t1, t2)) -> 
+          let sub = TArrow (TVar top, TVar (top+1)) in
+            unify_bnds (top+2) 
+                       (tSubst i sub ((TCons (t1, TVar top))::(TCons (TVar (top+1), t2))::xs)) 
+                       ((TCons (TVar i, sub))::(tSubst i sub subs))
+      | (TArrow (t1, t2), TVar i) -> 
+          let sub = TArrow (TVar top, TVar (top+1)) in
+            unify_bnds (top+2) 
+                       (tSubst i sub ((TCons (TVar top, t1))::(TCons (t2, TVar (top+1)))::xs)) 
+                       ((TCons (TVar i, sub))::(tSubst i sub subs))
+      | (TVar i, TVar j) -> unify_bnds top (xs @ [TCons (t1, t2)]) subs
+      | (TUnit, TUnit) -> unify_bnds top xs subs
+      | (TBool, TBool) -> unify_bnds top xs subs
+      | (TArray iexp, TArray iexp') -> unify_bnds top ((ICons (iexp', iexp))::xs) subs
+      | (TArrow (t1, t2), TArrow (s1, s2)) -> unify_bnds top ((TCons (s1, t1))::(TCons (t2, s2))::xs) subs
+      | _ -> None
+    end
+
+let rec unify_eq top eqs bnds subs = match eqs with
+  | [] -> unify_bnds top bnds subs
+  | (ICons (i1, i2))::xs ->
+    begin match (normalize i1, normalize i2) with
+      | (IVar i, iexp)
+      | (iexp, IVar i) -> unify_eq top (iSubst i iexp xs) (iSubst i iexp bnds) (iSubst i iexp subs)
+      | (ILit i, ILit j) -> if i = j then unify_eq top xs bnds subs else None
+      | (IPlus (IVar i, y), iexp) | (iexp, IPlus (IVar i, y)) ->
+        let sub = IPlus (IMinus y, iexp) in
+          unify_eq top (iSubst i sub eqs) (iSubst i sub bnds) (iSubst i sub subs)
+      | (IPlus (IMinus (IVar i), y), iexp) | (iexp, IPlus (IMinus (IVar i), y)) ->
+        let sub = IPlus (y, iexp) in
+          unify_eq top (iSubst i sub eqs) (iSubst i sub bnds) (iSubst i sub subs)
+      | _ -> None
+    end
+  | (TCons (t1, t2))::xs ->
+    begin match (t1, t2) with
+      | (TVar i, ty)
+      | (ty, TVar i) -> unify_eq top (tSubst i ty xs) (tSubst i ty bnds) ((TCons (TVar i, ty))::(tSubst i ty subs))
+      | (TUnit, TUnit) -> unify_eq top xs bnds subs
+      | (TBool, TBool) -> unify_eq top xs bnds subs
+      | (TArray iexp, TArray iexp') -> unify_eq top ((ICons (iexp, iexp'))::xs) bnds subs
+      | (TArrow (t1, t2), TArrow (s1, s2)) -> unify_eq top ((TCons (t1, s1))::(TCons (t2, s2))::xs) bnds subs
+      | _ -> None
+    end
+
+let rec applySubs subs tm = match subs with
+  | [] -> tm
+  | (TCons (TVar i, texp))::xs -> applySubs xs (substTyInGExpr tm i (toGType texp))
+  | _ -> failwith "impossible"
+
+let annotate tm =
+  let (top, eqs, bnds, typ) = inferTypes 0 [] tm in
+  let res = unify_eq top eqs bnds [] in
+    match res with
+      | None -> Err "Could not infer types"
+      | Some subs -> Val (applySubs subs tm)
