Makefile
@@ -3,7 +3,7 @@ FSTAR_HOME = /home/meamy/Programming/FStar
 FSTAR = $(FSTAR_HOME)/bin/fstar.exe
 FSHARP = fsharpc
 
-FILES = Set.fst Total.fst Partial.fst Util.fst PairHeap.fst AncillaHeap.fst Circuit.fst # BoolExp.fst ExprTypes.fst Interpreter.fst
+FILES = Set.fst Total.fst Partial.fst Util.fst PairHeap.fst AncillaHeap.fst Circuit.fst BoolExp.fst ExprTypes.fst #TypeCheck.fst Interpreter.fst
 #FILES = Util.fst Maps.fst PairHeap.fst AncillaHeap.fst Circuit.fst BoolExp.fst ExprTypes.fst Interpreter.fst
 REVS  = GenOp.fs Examples.fs Program.fs
 SUPPORT = FStar.Set FStar.Heap FStar.ST FStar.All FStar.List FStar.String FStar.IO
@@ -20,7 +20,7 @@ DLLS = $(FSTAR_HOME)/lib/fs/fstarlib.dll $(FSTAR_HOME)/bin/FSharp.PowerPack.dll 
 FSOPS = $(addprefix -r , $(DLLS))
 
 verify: $(FSTSRC)
-	$(FSTAR) --z3timeout 30 $^
+	$(FSTAR) --z3timeout 5 $^ --verify_module ExprTypes
 
 fs: $(FSTSRC)
 	$(FSTAR) --admit_smt_queries true --codegen FSharp $(EXCL) $^
